trying to give finite tuple domain. tuples are now represented as abstract locations, where injTuple makes the choice of which abstract location to put the tuple at. currently not fully implemented.

src/Analyze/AbstractDomains.v
@@ -54,9 +54,10 @@ Section AbstractDomain.
   ; applyA : forall {m} {_ : Monad m} {_ : MonadTrace string m}, (C -> D -> exp -> m D%type) -> D -> V -> list V -> list V -> m D%type
   }.
 
-  Class TplValue (V : Type) : Type :=
-  { injTuple : list V -> V
-  ; projA    : V -> V -> V
+  Require Import ExtLib.Data.Map.FMapAList.
+  Class TplValue (V : Type) (HV : Type) : Type :=
+  { injTuple : forall {m} {a : Monad m} {b : MonadState (alist var HV) m}, var -> list V -> V
+  ; projA    : forall {m} {a : Monad m} {b : MonadState (alist var HV) m}, V -> V -> V
   }.
 
 End AbstractDomain.
